Prefix(:=<http://www.ease-crc.org/ont/cram_failures.owl#>)
Prefix(DUL:=<http://www.ontologydesignpatterns.org/ont/dul/DUL.owl#>)
Prefix(owl:=<http://www.w3.org/2002/07/owl#>)
Prefix(rdf:=<http://www.w3.org/1999/02/22-rdf-syntax-ns#>)
Prefix(xml:=<http://www.w3.org/XML/1998/namespace>)
Prefix(xsd:=<http://www.w3.org/2001/XMLSchema#>)
Prefix(EASE:=<http://www.ease-crc.org/ont/EASE.owl#>)
Prefix(rdfs:=<http://www.w3.org/2000/01/rdf-schema#>)


Ontology(<http://www.ease-crc.org/ont/cram_failures.owl>
Import(<http://www.ease-crc.org/ont/failure_and_recovery.owl>)

Declaration(Class(:CRAMActionlibActionTimeout))
Declaration(Class(:CRAMDeliveringFailed))
Declaration(Class(:CRAMEnvironmentManipulationGoalNotReached))
Declaration(Class(:CRAMEnvironmentManipulationImpossible))
Declaration(Class(:CRAMEnvironmentUnreachable))
Declaration(Class(:CRAMFailureDiagnosis))
Declaration(Class(:CRAMFetchingFailed))
Declaration(Class(:CRAMGripperClosedCompletely))
Declaration(Class(:CRAMGripperGoalNotReached))
Declaration(Class(:CRAMGripperLowLevelFailure))
Declaration(Class(:CRAMHighLevelFailure))
Declaration(Class(:CRAMLookingHighLevelFailure))
Declaration(Class(:CRAMLowLevelFailure))
Declaration(Class(:CRAMManipulationGoalInCollision))
Declaration(Class(:CRAMManipulationGoalNotReached))
Declaration(Class(:CRAMManipulationLowLevelFailure))
Declaration(Class(:CRAMManipulationPoseUnreachable))
Declaration(Class(:CRAMNavigationGoalInCollision))
Declaration(Class(:CRAMNavigationGoalNotReached))
Declaration(Class(:CRAMNavigationHighLevelFailure))
Declaration(Class(:CRAMNavigationLowLevelFailure))
Declaration(Class(:CRAMNavigationPoseUnreachable))
Declaration(Class(:CRAMObjectNowhereToBeFound))
Declaration(Class(:CRAMObjectUndeliverable))
Declaration(Class(:CRAMObjectUnfetchable))
Declaration(Class(:CRAMObjectUnreachable))
Declaration(Class(:CRAMPerceptionLowLevelFailure))
Declaration(Class(:CRAMPerceptionObjectNotFound))
Declaration(Class(:CRAMPerceptionObjectNotInWorld))
Declaration(Class(:CRAMSearchingFailed))
Declaration(Class(:CRAMTorsoGoalNotReached))
Declaration(Class(:CRAMTorsoGoalUnreachable))
Declaration(Class(:CRAMTorsoLowLevelFailure))



############################
#   Classes
############################

# Class: :CRAMActionlibActionTimeout (:CRAMActionlibActionTimeout)

SubClassOf(:CRAMActionlibActionTimeout :CRAMLowLevelFailure)
SubClassOf(:CRAMActionlibActionTimeout ObjectSomeValuesFrom(DUL:describes ObjectSomeValuesFrom(DUL:isClassifiedBy <http://www.ease-crc.org/ont/failure_and_recovery.owl#Timeout>)))

# Class: :CRAMDeliveringFailed (:CRAMDeliveringFailed)

AnnotationAssertion(rdfs:comment :CRAMDeliveringFailed "Thrown when delivering plan completely gives up.")
SubClassOf(:CRAMDeliveringFailed :CRAMHighLevelFailure)
SubClassOf(Annotation(rdfs:comment "The main message of this error signal is that a particular CRAM plan (delivery) has exhausted its \"retry\" failure handling procedures and therefore one can conclude the error is of a sustained nature.") :CRAMDeliveringFailed ObjectSomeValuesFrom(DUL:describes ObjectSomeValuesFrom(DUL:isClassifiedBy <http://www.ease-crc.org/ont/failure_and_recovery.owl#SustainedFailure>)))

# Class: :CRAMEnvironmentManipulationGoalNotReached (:CRAMEnvironmentManipulationGoalNotReached)

AnnotationAssertion(rdfs:comment :CRAMEnvironmentManipulationGoalNotReached "Thrown when door / drawer opening / closing goal is still not reached.")
SubClassOf(:CRAMEnvironmentManipulationGoalNotReached :CRAMManipulationLowLevelFailure)
SubClassOf(:CRAMEnvironmentManipulationGoalNotReached ObjectSomeValuesFrom(DUL:describes ObjectSomeValuesFrom(DUL:isClassifiedBy <http://www.ease-crc.org/ont/failure_and_recovery.owl#ConfigurationNotReached>)))

# Class: :CRAMEnvironmentManipulationImpossible (:CRAMEnvironmentManipulationImpossible)

AnnotationAssertion(rdfs:comment :CRAMEnvironmentManipulationImpossible "Thrown when environment manipulation cannot be achieved.")
SubClassOf(:CRAMEnvironmentManipulationImpossible :CRAMHighLevelFailure)
SubClassOf(:CRAMEnvironmentManipulationImpossible ObjectSomeValuesFrom(DUL:describes ObjectSomeValuesFrom(DUL:isClassifiedBy ObjectUnionOf(<http://www.ease-crc.org/ont/failure_and_recovery.owl#CapabilityAbsenceFailure> <http://www.ease-crc.org/ont/failure_and_recovery.owl#ConfigurationNotReached>))))

# Class: :CRAMEnvironmentUnreachable (:CRAMEnvironmentUnreachable)

AnnotationAssertion(rdfs:comment :CRAMEnvironmentUnreachable "Thrown when environment manipulation in collision or unreachable.")
SubClassOf(:CRAMEnvironmentUnreachable :CRAMHighLevelFailure)
SubClassOf(:CRAMEnvironmentUnreachable ObjectSomeValuesFrom(DUL:describes ObjectSomeValuesFrom(DUL:isClassifiedBy <http://www.ease-crc.org/ont/failure_and_recovery.owl#ReachabilityFailure>)))

# Class: :CRAMFailureDiagnosis (:CRAMFailureDiagnosis)

AnnotationAssertion(rdfs:comment :CRAMFailureDiagnosis "A failure diagnosis evoked by one of the error conditions of the Cognitive Robot Abstract Machine (CRAM).")
SubClassOf(:CRAMFailureDiagnosis <http://www.ease-crc.org/ont/failure_and_recovery.owl#FailureDiagnosis>)

# Class: :CRAMFetchingFailed (:CRAMFetchingFailed)

AnnotationAssertion(rdfs:comment :CRAMFetchingFailed "Thrown when fetching plan completely gives up.")
SubClassOf(:CRAMFetchingFailed :CRAMHighLevelFailure)
SubClassOf(Annotation(rdfs:comment "The main message of this error signal is that a particular CRAM plan (fetch) has exhausted its \"retry\" failure handling procedures and therefore one can conclude the error is of a sustained nature.") :CRAMFetchingFailed ObjectSomeValuesFrom(DUL:describes ObjectSomeValuesFrom(DUL:isClassifiedBy <http://www.ease-crc.org/ont/failure_and_recovery.owl#SustainedFailure>)))

# Class: :CRAMGripperClosedCompletely (:CRAMGripperClosedCompletely)

AnnotationAssertion(rdfs:comment :CRAMGripperClosedCompletely "Thrown when the gripper closed completely, despite not being expected to do so (e.g. because it should have grasped something).")
SubClassOf(:CRAMGripperClosedCompletely :CRAMGripperLowLevelFailure)
SubClassOf(:CRAMGripperClosedCompletely ObjectSomeValuesFrom(DUL:describes ObjectSomeValuesFrom(DUL:isClassifiedBy <http://www.ease-crc.org/ont/failure_and_recovery.owl#ConfigurationNotReached>)))

# Class: :CRAMGripperGoalNotReached (:CRAMGripperGoalNotReached)

AnnotationAssertion(rdfs:comment :CRAMGripperGoalNotReached "Thrown when the gripper does not reach its goal.")
SubClassOf(:CRAMGripperGoalNotReached :CRAMGripperLowLevelFailure)
SubClassOf(:CRAMGripperGoalNotReached ObjectSomeValuesFrom(DUL:describes ObjectSomeValuesFrom(DUL:isClassifiedBy <http://www.ease-crc.org/ont/failure_and_recovery.owl#ConfigurationNotReached>)))

# Class: :CRAMGripperLowLevelFailure (:CRAMGripperLowLevelFailure)

AnnotationAssertion(rdfs:comment :CRAMGripperLowLevelFailure "Thrown when a failure involving the gripper hardware occurs.")
SubClassOf(:CRAMGripperLowLevelFailure :CRAMLowLevelFailure)
SubClassOf(:CRAMGripperLowLevelFailure ObjectSomeValuesFrom(DUL:describes ObjectSomeValuesFrom(DUL:isClassifiedBy <http://www.ease-crc.org/ont/failure_and_recovery.owl#EndEffectorFailure>)))

# Class: :CRAMHighLevelFailure (:CRAMHighLevelFailure)

AnnotationAssertion(rdfs:comment :CRAMHighLevelFailure "Failure thrown by high-level modules, i.e. plans.")
SubClassOf(:CRAMHighLevelFailure :CRAMFailureDiagnosis)

# Class: :CRAMLookingHighLevelFailure (:CRAMLookingHighLevelFailure)

AnnotationAssertion(rdfs:comment :CRAMLookingHighLevelFailure "High-level failure produced when looking for an object, i.e. it is not a hardware issue but one relating to the looking task, its parameters, and how they relate to the environment.")
SubClassOf(:CRAMLookingHighLevelFailure :CRAMHighLevelFailure)
SubClassOf(:CRAMLookingHighLevelFailure ObjectSomeValuesFrom(DUL:describes ObjectSomeValuesFrom(DUL:isClassifiedBy <http://www.ease-crc.org/ont/failure_and_recovery.owl#ObjectNotFound>)))

# Class: :CRAMLowLevelFailure (:CRAMLowLevelFailure)

AnnotationAssertion(rdfs:comment :CRAMLowLevelFailure "Failure thrown by low-level modules: robot or projection PMs.")
SubClassOf(:CRAMLowLevelFailure :CRAMFailureDiagnosis)

# Class: :CRAMManipulationGoalInCollision (:CRAMManipulationGoalInCollision)

AnnotationAssertion(rdfs:comment :CRAMManipulationGoalInCollision "Thrown when executing a manipulation action results in a collision.")
SubClassOf(:CRAMManipulationGoalInCollision :CRAMHighLevelFailure)
SubClassOf(:CRAMManipulationGoalInCollision ObjectSomeValuesFrom(DUL:describes ObjectSomeValuesFrom(DUL:isClassifiedBy <http://www.ease-crc.org/ont/failure_and_recovery.owl#IllPosedGoalFailure>)))

# Class: :CRAMManipulationGoalNotReached (:CRAMManipulationGoalNotReached)

AnnotationAssertion(rdfs:comment :CRAMManipulationGoalNotReached "Thrown when after executing the action, goal is still not reached.")
SubClassOf(:CRAMManipulationGoalNotReached :CRAMManipulationLowLevelFailure)
SubClassOf(:CRAMManipulationGoalNotReached ObjectSomeValuesFrom(DUL:describes ObjectSomeValuesFrom(DUL:isClassifiedBy <http://www.ease-crc.org/ont/failure_and_recovery.owl#ConfigurationNotReached>)))

# Class: :CRAMManipulationLowLevelFailure (:CRAMManipulationLowLevelFailure)

AnnotationAssertion(rdfs:comment :CRAMManipulationLowLevelFailure "Thrown when a low-level, i.e. hardware related, failure is detected in a manipulation action.")
SubClassOf(:CRAMManipulationLowLevelFailure :CRAMLowLevelFailure)
SubClassOf(:CRAMManipulationLowLevelFailure ObjectSomeValuesFrom(DUL:describes ObjectSomeValuesFrom(DUL:isClassifiedBy <http://www.ease-crc.org/ont/failure_and_recovery.owl#ArmFailure>)))

# Class: :CRAMManipulationPoseUnreachable (:CRAMManipulationPoseUnreachable)

AnnotationAssertion(rdfs:comment :CRAMManipulationPoseUnreachable "Thrown when no IK solution can be found.")
SubClassOf(:CRAMManipulationPoseUnreachable :CRAMManipulationLowLevelFailure)
SubClassOf(:CRAMManipulationPoseUnreachable ObjectSomeValuesFrom(DUL:describes ObjectSomeValuesFrom(DUL:isClassifiedBy <http://www.ease-crc.org/ont/failure_and_recovery.owl#ReachabilityFailure>)))

# Class: :CRAMNavigationGoalInCollision (:CRAMNavigationGoalInCollision)

AnnotationAssertion(rdfs:comment :CRAMNavigationGoalInCollision "Navigation goal cannot be reached because the goal itself is already occupied by some other object.")
SubClassOf(:CRAMNavigationGoalInCollision :CRAMNavigationHighLevelFailure)
SubClassOf(:CRAMNavigationGoalInCollision ObjectSomeValuesFrom(DUL:describes ObjectSomeValuesFrom(DUL:isClassifiedBy <http://www.ease-crc.org/ont/failure_and_recovery.owl#IllPosedGoalFailure>)))

# Class: :CRAMNavigationGoalNotReached (:CRAMNavigationGoalNotReached)

AnnotationAssertion(rdfs:comment :CRAMNavigationGoalNotReached "Thrown when the base moved as a result of the navigation action but the goal was not reached.")
SubClassOf(:CRAMNavigationGoalNotReached :CRAMNavigationLowLevelFailure)
SubClassOf(:CRAMNavigationGoalNotReached ObjectSomeValuesFrom(DUL:describes ObjectSomeValuesFrom(DUL:isClassifiedBy <http://www.ease-crc.org/ont/failure_and_recovery.owl#ConfigurationNotReached>)))

# Class: :CRAMNavigationHighLevelFailure (:CRAMNavigationHighLevelFailure)

AnnotationAssertion(rdfs:comment :CRAMNavigationHighLevelFailure "High-level failure produced while navigating the robot, i.e. it is not a hardware issue but one relating to the navigation task, its parameters, and how they relate to the environment.")
SubClassOf(:CRAMNavigationHighLevelFailure :CRAMHighLevelFailure)

# Class: :CRAMNavigationLowLevelFailure (:CRAMNavigationLowLevelFailure)

AnnotationAssertion(rdfs:comment :CRAMNavigationLowLevelFailure "Low-level failure produced while navigating the robot, i.e. some kind of hardware issue.")
SubClassOf(:CRAMNavigationLowLevelFailure :CRAMLowLevelFailure)
SubClassOf(:CRAMNavigationLowLevelFailure ObjectSomeValuesFrom(DUL:describes ObjectSomeValuesFrom(DUL:isClassifiedBy <http://www.ease-crc.org/ont/failure_and_recovery.owl#LocomotorFailure>)))

# Class: :CRAMNavigationPoseUnreachable (:CRAMNavigationPoseUnreachable)

AnnotationAssertion(rdfs:comment :CRAMNavigationPoseUnreachable "Thrown when the goal pose for navigation is computed to be unreachable.")
SubClassOf(:CRAMNavigationPoseUnreachable :CRAMNavigationLowLevelFailure)
SubClassOf(:CRAMNavigationPoseUnreachable ObjectSomeValuesFrom(DUL:describes ObjectSomeValuesFrom(DUL:isClassifiedBy <http://www.ease-crc.org/ont/failure_and_recovery.owl#ReachabilityFailure>)))

# Class: :CRAMObjectNowhereToBeFound (:CRAMObjectNowhereToBeFound)

AnnotationAssertion(rdfs:comment :CRAMObjectNowhereToBeFound "Thrown when the robot cannot find an object of a given description in its surroundings.")
SubClassOf(:CRAMObjectNowhereToBeFound :CRAMHighLevelFailure)
SubClassOf(:CRAMObjectNowhereToBeFound ObjectSomeValuesFrom(DUL:describes ObjectSomeValuesFrom(DUL:isClassifiedBy <http://www.ease-crc.org/ont/failure_and_recovery.owl#ObjectUnavailable>)))

# Class: :CRAMObjectUndeliverable (:CRAMObjectUndeliverable)

AnnotationAssertion(rdfs:comment :CRAMObjectUndeliverable "Thrown when no base positioning can assure a reachable pose to place the object from.")
SubClassOf(:CRAMObjectUndeliverable :CRAMHighLevelFailure)
SubClassOf(:CRAMObjectUndeliverable ObjectSomeValuesFrom(DUL:describes ObjectSomeValuesFrom(DUL:isClassifiedBy <http://www.ease-crc.org/ont/failure_and_recovery.owl#ReachabilityFailure>)))

# Class: :CRAMObjectUnfetchable (:CRAMObjectUnfetchable)

AnnotationAssertion(rdfs:comment :CRAMObjectUnfetchable "Thrown when no base positioning can assure a reachable pose to grasp the object from.")
SubClassOf(:CRAMObjectUnfetchable :CRAMHighLevelFailure)
SubClassOf(:CRAMObjectUnfetchable ObjectSomeValuesFrom(DUL:describes ObjectSomeValuesFrom(DUL:isClassifiedBy <http://www.ease-crc.org/ont/failure_and_recovery.owl#ReachabilityFailure>)))

# Class: :CRAMObjectUnreachable (:CRAMObjectUnreachable)

AnnotationAssertion(rdfs:comment :CRAMObjectUnreachable "Thrown when no IK found for particular base pose.")
SubClassOf(:CRAMObjectUnreachable :CRAMHighLevelFailure)
SubClassOf(:CRAMObjectUnreachable ObjectSomeValuesFrom(DUL:describes ObjectSomeValuesFrom(DUL:isClassifiedBy <http://www.ease-crc.org/ont/failure_and_recovery.owl#ReachabilityFailure>)))

# Class: :CRAMPerceptionLowLevelFailure (:CRAMPerceptionLowLevelFailure)

AnnotationAssertion(rdfs:comment :CRAMPerceptionLowLevelFailure "Low-level failure produced while perceiving, i.e. some kind of hardware issue.")
SubClassOf(:CRAMPerceptionLowLevelFailure :CRAMLowLevelFailure)
SubClassOf(:CRAMPerceptionLowLevelFailure ObjectSomeValuesFrom(DUL:describes ObjectSomeValuesFrom(DUL:isClassifiedBy <http://www.ease-crc.org/ont/failure_and_recovery.owl#SensorFailure>)))

# Class: :CRAMPerceptionObjectNotFound (:CRAMPerceptionObjectNotFound)

AnnotationAssertion(rdfs:comment :CRAMPerceptionObjectNotFound "Thrown when an attempt to find an object by perception fails -- and this can still be interpreted as the robot not looking in the right direction, as opposed to the object being absent.")
SubClassOf(:CRAMPerceptionObjectNotFound :CRAMPerceptionLowLevelFailure)
SubClassOf(:CRAMPerceptionObjectNotFound ObjectSomeValuesFrom(DUL:describes ObjectSomeValuesFrom(DUL:isClassifiedBy <http://www.ease-crc.org/ont/failure_and_recovery.owl#ObjectNotFound>)))

# Class: :CRAMPerceptionObjectNotInWorld (:CRAMPerceptionObjectNotInWorld)

AnnotationAssertion(rdfs:comment :CRAMPerceptionObjectNotInWorld "Thrown when an attempt to find an object by perception fails -- and this is because the object can be assumed absent or perhaps is known absent because of the setup of a simulation.")
SubClassOf(:CRAMPerceptionObjectNotInWorld :CRAMPerceptionLowLevelFailure)
SubClassOf(:CRAMPerceptionObjectNotInWorld ObjectSomeValuesFrom(DUL:describes ObjectSomeValuesFrom(DUL:isClassifiedBy <http://www.ease-crc.org/ont/failure_and_recovery.owl#ObjectUnavailable>)))

# Class: :CRAMSearchingFailed (:CRAMSearchingFailed)

AnnotationAssertion(rdfs:comment :CRAMSearchingFailed "Thrown when searching plan completely gives up.")
SubClassOf(:CRAMSearchingFailed :CRAMHighLevelFailure)
SubClassOf(Annotation(rdfs:comment "The main message of this error signal is that a particular CRAM plan (search) has exhausted its \"retry\" failure handling procedures and therefore one can conclude the error is of a sustained nature.") :CRAMSearchingFailed ObjectSomeValuesFrom(DUL:describes ObjectSomeValuesFrom(DUL:isClassifiedBy <http://www.ease-crc.org/ont/failure_and_recovery.owl#SustainedFailure>)))

# Class: :CRAMTorsoGoalNotReached (:CRAMTorsoGoalNotReached)

AnnotationAssertion(rdfs:comment :CRAMTorsoGoalNotReached "Thrown when the torso moved as a result of a torso action but the goal was not reached.")
SubClassOf(:CRAMTorsoGoalNotReached :CRAMTorsoLowLevelFailure)
SubClassOf(:CRAMTorsoGoalNotReached ObjectSomeValuesFrom(DUL:describes ObjectSomeValuesFrom(DUL:isClassifiedBy <http://www.ease-crc.org/ont/failure_and_recovery.owl#ConfigurationNotReached>)))

# Class: :CRAMTorsoGoalUnreachable (:CRAMTorsoGoalUnreachable)

AnnotationAssertion(rdfs:comment :CRAMTorsoGoalUnreachable "Thrown when the goal for the torso is computed to be unreachable.")
SubClassOf(:CRAMTorsoGoalUnreachable :CRAMTorsoLowLevelFailure)
SubClassOf(:CRAMTorsoGoalUnreachable ObjectSomeValuesFrom(DUL:describes ObjectSomeValuesFrom(DUL:isClassifiedBy <http://www.ease-crc.org/ont/failure_and_recovery.owl#ReachabilityFailure>)))

# Class: :CRAMTorsoLowLevelFailure (:CRAMTorsoLowLevelFailure)

AnnotationAssertion(rdfs:comment :CRAMTorsoLowLevelFailure "Low-level failure produced while moving the torso, i.e. some kind of hardware issue.")
SubClassOf(:CRAMTorsoLowLevelFailure :CRAMLowLevelFailure)
SubClassOf(:CRAMTorsoLowLevelFailure ObjectSomeValuesFrom(DUL:describes ObjectSomeValuesFrom(DUL:isClassifiedBy <http://www.ease-crc.org/ont/failure_and_recovery.owl#TorsoFailure>)))


AnnotationAssertion(rdfs:comment :CRAMActionlibActionTimedout "Actionlib action timeout was reached.")
)